---
title: Detailed Proof of IPW Identification
description: ${\scriptstyle E[Y(1)-Y(0)] \\ = E[\frac{\mathbb{1}(T=1)Y}{e(W)}]-E[\frac{\mathbb{1}(T=0)Y}{1-e(W)}]}$
author:
  - name: Jia Zhang
    url: https://jiazhang42.github.io/mysite/ 
    #affiliation: 
    #affiliation-url:
date: 01-05-2023
categories: [Causal Inference] # self-defined categories
citation: 
  url: https://jiazhang42.github.io/mysite/blog/ipw/ 
#image: frontdoor.jpg
draft: false # setting this to `true` will prevent your post from appearing on your listing page until you're ready!
#bibliography: references.bib
---

We need to prove that under unconfoundedness and positivity,

$EY(t) = E\frac{\mathbb{1}(T=t)Y}{P(t|W)}.$

::: callout-note
## Proof

$$
\begin{split}
EY(t) &= E(Y|do(t))\\
&= EE(Y|do(t), W)\\
&= EE(Y|t, W)\\
&= \Sigma_w E(Y|t, w) P(w)\\
&= \Sigma_w \Sigma_y y P(y|t,w) P(w)\\
&= \Sigma_w \Sigma_y y \frac{P(y,t,w)}{P(t,w)} P(w)\\
&= \Sigma_w \Sigma_y y P(y,t,w)\frac{1}{P(t|w)}\\
&= \Sigma_w \Sigma_y y E(\mathbb{1}(Y=y,T=t,W=w))\frac{1}{P(t|w)}\\
&= \Sigma_w E(\Sigma_y y \mathbb{1}(Y=y) \mathbb{1}(T=t,W=w))\frac{1}{P(t|w)}\\
&= \Sigma_w E(Y \mathbb{1}(T=t,W=w))\frac{1}{P(t|w)}\\
&= E(Y \mathbb{1}(T=t) \Sigma_w \mathbb{1}(W=w)\frac{1}{P(t|w)})\\
&= E(Y \mathbb{1}(T=t) \frac{1}{P(t|W)})
\end{split}
$$
:::

Note that we used the following properties of the indicator function:

-   $$
    E\mathbb{1}(X=x) = P(X=x)
    $$

-   $$
    \mathbb{1}(X=x, Y=y) = \mathbb{1}(X=x) \mathbb{1}(Y=y)
    $$

-   $$
    \Sigma_x \mathbb{1}(X=x)f(x) = f(X)
    $$
